

Final Exam

Brandon Keck, ID:qh9701

2024-12-11

1.

(a)

$$L(\theta; y_1, y_2, \dots, y_n) = \prod_{i=1}^n f(y_i; \theta) = (\theta + 1)^n \prod_{i=1}^n y_i^\theta$$
$$\ln(\theta) = n \ln(\theta + 1) + \theta \sum_{i=1}^n \ln(y_i)$$
$$\frac{d}{d\theta} = \frac{n}{\theta + 1} + \sum_{i=1}^n \ln(y_i)$$
$$\frac{n}{\theta + 1} + \sum_{i=1}^n \ln(y_i) = 0$$
$$\theta + 1 = - \frac{n}{\sum_{i=1}^n \ln(y_i)}$$
$$\theta = - \frac{n}{\sum_{i=1}^n \ln(y_i)} - 1$$

$$\hat{\theta} = - \frac{n}{\sum_{i=1}^n \ln(y_i)} - 1$$

(b)

$$E(Y) = \int_0^1 y * (\theta + 1) y^\theta dy$$
$$E(Y) = (\theta + 1) \int_0^1 y^{\theta+1} dy = (\theta + 1) * \frac{1}{\theta + 2}$$
$$E(Y) = \frac{\theta + 1}{\theta + 2}$$
$$\hat{Y} = \frac{\theta + 1}{\theta + 2}$$
$$\hat{Y}(\theta + 2) = \theta + 1$$
$$\hat{Y}\theta + 2\hat{Y} = \theta + 1$$
$$\hat{Y}\theta - \theta = 1 - 2\hat{Y}$$
$$\theta(\hat{Y} - 1) = 1 - 2\hat{Y}$$

$$\hat{\theta} = \frac{1 - 2\hat{Y}}{\hat{Y} - 1}$$

(c)

$$\hat{Y} = \frac{\sum_{i=1}^{1000} y_i}{1000}$$

750.7516 / 1000
[1] 0.7507516
$\hat{\theta} = - \frac{n}{\sum_{i=1}^n \ln(y_i)} - 1$
1000 / -329.0056
[1] -3.039462
-(-3.039462)
[1] 3.039462
3.039462 - 1
[1] 2.039462
$\hat{\theta} = 2.039462$
$\hat{\theta} = \frac{1 - 2\hat{Y}}{\hat{Y} - 1}$
(1 - 2 * 0.7507516) / (0.7507516 - 1)
[1] 2.012062
$\hat{\theta} = 2.012062$

2.

(a)

$$f_{XY}(x,y) = 6(1-y), \ 0 \leq x \leq y \leq 1.$$
$$P(X \leq \frac{3}{4}, Y > \frac{1}{2})$$
$$= \int_{\frac{1}{2}}^1 \int_0^{\frac{1}{2}} 6(1-y) dx dy$$
$$= \int_{\frac{1}{2}}^{\frac{1}{2}} \int_0^y 6(1-y) dx dy + \int_{\frac{1}{2}}^1 \int_0^{\frac{1}{2}} 6(1-y) dx dy$$

First Region:

$$\int_{\frac{1}{2}}^{\frac{1}{2}} \int_0^y 6(1-y) dx dy = \int_{\frac{1}{2}}^{\frac{1}{2}} [6(1-y)x]_0^y dy$$
$$= \int_{\frac{1}{2}}^{\frac{1}{2}} 6(1-y)y dy$$
$$= 6 \int_{\frac{1}{2}}^{\frac{1}{2}} (1-y)y dy$$
$$= 6[\frac{y^2}{2} - \frac{y^3}{3}]_{\frac{1}{2}}^{\frac{1}{2}}$$
$$= 6[\frac{(\frac{1}{2})^2}{2} - \frac{(\frac{1}{2})^3}{3}] - [\frac{(\frac{1}{2})^2}{2} - \frac{(\frac{1}{2})^3}{3}]$$
$$= 6[\frac{9}{32} - \frac{27}{192}] - [\frac{1}{8} - \frac{1}{24}]$$
$$= \frac{11}{32}$$

First region = $\frac{11}{32}$

Second Region:

$$= \int_{\frac{1}{2}}^1 \int_0^{\frac{1}{2}} 6(1-y) dx dy$$
$$= \int_{\frac{1}{2}}^1 [6(1-y)x]_0^{\frac{1}{2}} dy$$
$$= \int_{\frac{1}{2}}^1 6(1-y)(\frac{3}{4}) dy$$
$$= \frac{18}{4} [y - \frac{y^2}{2}]_{\frac{1}{2}}^1$$
$$= \frac{18}{4} [1 - \frac{1}{2}] - [\frac{3}{4} - \frac{(\frac{1}{2})^2}{2}]$$
$$= \frac{18}{4} [\frac{1}{2} - \frac{15}{32}]$$

Region2 = $\frac{9}{64}$

11/32 + 9/64
[1] 0.484375
0.484375

(b)

Find the Marginal density function of X.

$$f_X(x) = f_{XY}(x,y) dy$$
$$f_X(x) = \int_{y=x}^1 6(1-y) dy$$
$$= 6 \int_{y=x}^1 (1-y) dy$$
$$= 6(y - \frac{y^2}{2})_{y=x}^1$$
$$= 6[(1 - \frac{1}{2}) - (x - \frac{x^2}{2})]$$
$$= 6(\frac{1}{2}) - (x - \frac{x^2}{2})$$
$$= 6[\frac{1}{2} - x + \frac{x^2}{2}]$$
$$= 3 - 6x + 3x^2$$

$$f_X(x) = 3 - 6x + 3x^2, \ 0 \leq x \leq 1$$

(c)

$$E(X) = \int_0^1 x * f_X(x) dx$$
$$E(X) = \int_0^1 x * (3 - 6x + 3x^2) dx$$
$$= \int_0^1 (3x - 6x^2 + 3x^3) dx$$
$$= \frac{3x^2}{2} - \frac{6x^3}{3} + \frac{3x^4}{4} \Big|_0^1$$
$$= \frac{3(1)^2}{2} - \frac{6(1)^3}{3} + \frac{3(1)^4}{4}$$

3/2 - 6/3 + 3/4
[1] 0.25
E(X) = 0.25

To calculate the Var(X) we first compute $E(X^2)$

$$E(X^2) = \int_0^1 x^2 * f_X(x) dx$$
$$E(X) = \int_0^1 x^2 * (3 - 6x + 3x^2) dx$$
$$= \int_0^1 (3x^2 - 6x^3 + 3x^4) dx$$
$$= \frac{3x^3}{3} - \frac{6x^4}{4} + \frac{3x^5}{5} \Big|_0^1$$

1 - 6/4 + 3/5
[1] 0.1
Var(X) = E(X^2) - [E(X)]^2
0.1 - (0.25)^2
[1] 0.0375
Var(X) = 0.0375

3.

(a)

Conditions for Independence

$$P(X = x, Y = y) = P_X(x) * P_Y(y)$$

Marginal PMF of X

$$P_X(x) = \sum_y P(X = x, Y = y)$$
$$X = 1 : P_X(1) = 0.1 + 0.1 = 0.2$$
$$X = 2 : P_X(2) = 0.3 + 0.3 = 0.6$$
$$X = 3 : P_X(3) = 0.1 + 0.1 = 0.2$$

Marginal PMF of Y

$$Y = 0 : P_Y(0) = 0.3$$
$$Y = 1 : P_Y(1) = 0.1 + 0.1 = 0.2$$
$$Y = 3 : P_Y(3) = 0.1 + 0.1 = 0.2$$
$$Y = 4 : P_Y(4) = 0.3$$

Check Independence:

$$P(2, 0) = P_X(2) * P_Y(0) = 0.6 * 0.3 = 0.18 \neq 0.3$$

X and Y are not independent

(b)

$$Let \ W = X^2(Y - 2)$$

X	Y	P(X,Y)	W = X ² (Y - 2)	W ²	W * P(X,Y)	W ² * P(X,Y)
2	0	0.30	2 ² (0 - 2) = -8	(-8) ² = 64	-8 * 0.30 = -2.4	64 * 0.30 = 19.2
1	1	0.10	1 ² (1 - 2) = -1	(-1) ² = 1	-1 * 0.10 = -0.1	1 * 0.10 = 0.1
2	4	0.30	2 ² (4 - 2) = 8	(8) ² = 64	8 * 0.30 = 2.4	64 * 0.30 = 19.2
1	3	0.10	1 ² (3 - 2) = 1	(1) ² = 1	1 * 0.10 = 0.10	1 * 0.10 = 0.10
3	1	0.10	3 ² (1 - 2) = -9	(-9) ² = 81	-9 * 0.10 = -0.9	81 * 0.10 = 8.1
3	3	0.10	3 ² (3 - 2) = 9	(9) ² = 81	9 * 0.10 = 0.9	81 * 0.10 = 8.1

$$E(W) = \sum W * P(X,Y)$$

-2.4 + (-0.1) + 2.4 + 0.10 + (-0.9) + 0.9
[1] -1.110223e-16
$E(W^2) = \sum W^2 * P(X,Y)$
19.2 + 0.10 + 19.2 + 0.10 + 8.1 + 8.1
[1] 54.8

$$Var(W) = E(W^2) - [E(W)]^2$$

$$54.8 - 0 = 54.8$$

Var(W) = 54.8

(c)

P(W>0)

$$W = X^2(Y - 2) > 0$$
$$X^2 > 0$$
$$Y - 2 > 0 \Rightarrow Y > 2$$

X	Y	P(X,Y)	W = X ² (Y - 2)
1	3	0.10	1 ² (3 - 2) = 1
2	4	0.30	2 ² (4 - 2) = 8
3	3	0.10	3 ² (3 - 2) = 9

$$P(W > 0) = P(1, 3) + P(2, 4) + P(3, 3) = 0.10 + 0.30 + 0.10 = 0.50$$

P(W > 0) = 0.50

4.

(a)

Find Var(X̂)

Given is Var(X) = 0.03 and n = 20

Formula for Var(X̂) = $\frac{\sigma^2}{n}$

0.03 / 20
[1] 0.0015
Var(X̂) = 0.0015

(b)

$$\mu_{\hat{X}} = E(X)$$
$$\sigma_{\hat{X}} = \sqrt{Var(\hat{X})} = \sqrt{\frac{Var(X)}{n}}$$

sqrt(0.03/20)
[1] 0.03872983
Standardize
$Z = \frac{\hat{X} - \mu_{\hat{X}}}{\sigma_{\hat{X}}}$
Z ₁
(3.39-3.5) / 0.03872983
[1] -2.840188
Z ₂
(3.6-3.5) / 0.03872983
[1] 2.581989

Standard Normal Table P(3.39 ≤ X̂ ≤ 3.6 = P(Z₁ ≤ X̂ ≤ Z₂

Z₁ = -2.840 = 0.0023

Z₂ = 2.58 = 0.9951

$$P(Z \leq 2.58) - P(Z \leq -2.84) = 0.9951 - 0.0023 \approx 0.9928$$

P(3.39 ≤ X̂ ≤ 3.6 ≈ 0.9928

(c)

Assumptions made: For the sampling distribution of X (GPA) if this is normal, the sampling distribution will also be normal regardless of the sample size. However, the CLT states that the sampling distribution will approximate a normal distribution as the sample size n becomes sufficiently large.

5.

(a)

$$M(t) = \sum_{x=1}^{10} e^{tx} cx$$
$$M(t) = c \sum_{x=1}^{10} x e^{tx} = 1$$
$$M(0) = c \sum_{x=1}^{10} x e^0 = 1$$
$$M(0) = c(1 + 2 + 3 + 4 + 5 + 6 + 7 + 8 + 9 + 10) = 1$$
$$c(55) = 1$$
$$c = \frac{1}{55}$$

E(X) is equal to the first derivative of the MGF

$$M'(t) = c \sum_{x=1}^{10} x^2 e^{tx} dt$$
$$M'(0) = \sum_{x=1}^{10} x^2 e^{0x} (\frac{1}{55})$$
$$= \sum_{x=1}^{10} x^2 * \frac{1}{55}$$

(1/55) * (1^2 + 2^2 + 3^2 + 4^2 + 5^2 + 6^2 + 7^2 + 8^2 + 9^2 + 10^2)
[1] 7
$E(X) = 7$
$M''(t) = c \sum_{x=1}^{10} x^3 e^{tx}$

Evaluate at t = 0

$$M''(0) = \sum_{x=1}^{10} cx^3$$
$$= \sum_{x=1}^{10} \frac{1}{55} * x^3$$

(1/55) * (1^3 + 2^3 + 3^3 + 4^3 + 5^3 + 6^3 + 7^3 + 8^3 + 9^3 + 10^3)
[1] 55
$Var(X) = E(X^2) - [E(X)]^2$
55 - (7^2)
[1] 6
$Var(X) = 6$

(b)

$$\sum_{x=1}^{10} P(X = x) = 1$$
$$\sum_{x=1}^{10} cx = 1$$

We found c = $\frac{1}{55}$

$$\sum_{x=1}^{10} P(X = x) = \sum_{x=1}^{10} \frac{x}{55} = \frac{1}{55} \sum_{x=1}^{10} x = \frac{1}{55} * 55 = 1$$

$$pmf \ of \ X : P(X = x) = \frac{x}{55}, x = 1, 2, 3, \dots, 10$$

(c)

Using the pmf of X P(X=x) = $\frac{x}{55}$, x = 1, 2, 3, ..., 10

$$P(X > 8) = P(X = 9) + P(X = 10)$$

$$P(X = 9) = \frac{9}{55}$$

$$P(X = 10) = \frac{10}{55}$$

9/55 + 10/55
[1] 0.3454545
$P(X > 8) = \frac{19}{55}$